feat: `simp`

src/Lean/Meta/Tactic/Simp/Main.lean
@@ -9,11 +9,121 @@ import Lean.Meta.Tactic.Simp.Rewrite
 namespace Lean.Meta
 namespace Simp
 
-def main (e : Expr) : M σ Result :=
-  return (← post e).result -- TODO: traverse term
+private def join (p₁? p₂? : Option Expr) : MetaM (Option Expr) :=
+  match p₁? with
+  | none    => return p₂?
+  | some p₁ => match p₂? with
+    | none    => return p₁?
+    | some p₂ => return some (← mkEqTrans p₁ p₂)
 
-def simp (e : Expr) (s : σ) (config : Config := {}) (methods : Methods σ := {}) (simpLemmas : SimpLemmas := {}) : MetaM Result := do
-  main e methods { config := config, simpLemmas := simpLemmas } |>.run' { user := s }
+mutual
+  partial def dsimp (e : Expr) : M σ Expr :=
+    return e -- TODO
+
+  partial def reduce (e : Expr) : M σ Expr :=
+    return e -- TODO
+
+  partial def simp {σ} (e : Expr) : M σ Result := withIncRecDepth do
+    let cfg ← getConfig
+    if cfg.memoize then
+      if let some result := (← get).cache.find? e then
+        return result
+    if (← get).numSteps > cfg.maxSteps then
+       throwError! "simp failed, maximum number of steps exceeded"
+    modify fun s => { s with numSteps := s.numSteps + 1 }
+    match (← pre e) with
+    | Step.done r => cacheResult cfg r
+    | Step.visit { expr := e, proof? := p } =>
+      let { expr := e, proof? := p' } ←
+        match e with
+        | Expr.mdata _ e _ => simp e
+        | Expr.proj ..     => simpProj e
+        | Expr.app ..      => simpApp e
+        | Expr.lam ..      => simpLambda e
+        | Expr.forallE ..  => simpForall e
+        | Expr.letE ..     => simpLet e
+        | Expr.const ..    => simpConst e
+        | Expr.bvar ..     => unreachable!
+        | Expr.sort ..     => pure { expr := e }
+        | Expr.lit ..      => pure { expr := e }
+        | Expr.mvar ..     => simpMVar e
+        | Expr.fvar ..     => simpFVar e
+      let p ← join p p'
+      match (← post e) with
+      | Step.done { expr := e, proof? := p' } => cacheResult cfg { expr := e, proof? := (← join p p') }
+      | Step.visit { expr := e', proof? := p' } =>
+        let p ← join p p'
+        if cfg.singlePass || e == e' then
+          cacheResult cfg { expr := e', proof? := p }
+        else
+          let { expr := e', proof? := p' } ← simp e'
+          cacheResult cfg { expr := e', proof? := (← join p p') }
+
+  where
+    simpProj (e : Expr) : M σ Result :=
+      return { expr := e } -- TODO
+
+    mkCongrFun (r : Result) (a : Expr) : MetaM Result :=
+      match r.proof? with
+      | none   => return { expr := mkApp r.expr a, proof? := none }
+      | some h => return { expr := mkApp r.expr a, proof? := (← Meta.mkCongrFun h a) }
+
+    mkCongr (r₁ r₂ : Result) : MetaM Result :=
+      let e := mkApp r₁.expr r₂.expr
+      match r₁.proof?, r₂.proof? with
+      | none,     none   => return { expr := e, proof? := none }
+      | some h,  none    => return { expr := e, proof? := (← Meta.mkCongrFun h r₂.expr) }
+      | none,    some h  => return { expr := e, proof? := (← Meta.mkCongrArg r₁.expr h) }
+      | some h₁, some h₂ => return { expr := e, proof? := (← Meta.mkCongr h₁ h₂) }
+
+    simpApp (e : Expr) : M σ Result := do
+      let e ← reduce e
+      if !e.isApp then
+        simp e
+      else
+        withParent e <| e.withApp fun f args => do
+          let infos := (← getFunInfoNArgs f args.size).paramInfo
+          let mut r ← simp f
+          let mut i := 0
+          for arg in args do
+            if i < infos.size && !infos[i].hasFwdDeps then
+              r ← mkCongr r (← simp arg)
+            else
+              r ← mkCongrFun r arg
+            i := i + 1
+          return r
+
+    simpLambda (e : Expr) : M σ Result :=
+      return { expr := e } -- TODO
+
+    simpForall (e : Expr) : M σ Result :=
+      return { expr := e } -- TODO
+
+    simpLet (e : Expr) : M σ Result :=
+      return { expr := e } -- TODO
+
+    simpConst (e : Expr) : M σ Result :=
+      return { expr := e } -- TODO
+
+    simpMVar (e : Expr) : M σ Result :=
+      return { expr := e } -- TODO
+
+    simpFVar (e : Expr) : M σ Result := do
+      if (← getConfig).zeta then
+        match (← getFVarLocalDecl e).value? with
+        | some v => simp v
+        | none   => return { expr := e }
+      else
+        return { expr := e }
+
+    cacheResult (cfg : Config) (r : Result) : M σ Result := do
+      if cfg.memoize then
+        modify fun s => { s with cache := s.cache.insert e r }
+      return r
+end
+
+def main (e : Expr) (s : σ) (config : Config := {}) (methods : Methods σ := {}) (simpLemmas : SimpLemmas := {}) : MetaM Result := do
+  simp e methods { config := config, simpLemmas := simpLemmas } |>.run' { user := s }
 
 end Simp
 
@@ -21,6 +131,6 @@ def simp (e : Expr) (simpLemmas : SimpLemmas := {}) : MetaM Simp.Result := do
   let discharge? (e : Expr) : SimpM Unit (Option Expr) := return none -- TODO: use simp, and add config option
   let pre  := (Simp.preDefault · discharge?)
   let post := (Simp.postDefault · discharge?)
-  Simp.simp e () (methods := { pre := pre, post := post, discharge? := discharge? }) (simpLemmas := simpLemmas)
+  Simp.main e () (methods := { pre := pre, post := post, discharge? := discharge? }) (simpLemmas := simpLemmas)
 
 end Lean.Meta
