src/Lean/Meta/Tactic/Simp/Types.lean
@@ -3,6 +3,7 @@ Copyright (c) 2020 Microsoft Corporation. All rights reserved.
 Released under Apache 2.0 license as described in the file LICENSE.
 Authors: Leonardo de Moura
 -/
+import Lean.Meta.AppBuilder
 import Lean.Meta.Tactic.Simp.SimpLemmas
 
 namespace Lean.Meta
@@ -13,6 +14,7 @@ def defaultMaxSteps := 100000
 structure Result where
   expr   : Expr
   proof? : Option Expr := none -- If none, proof is assumed to be `refl`
+  deriving Inhabited
 
 abbrev Cache := ExprMap Result
 
@@ -63,6 +65,12 @@ def post (e : Expr) : M σ Step := do
 
 def discharge? (e : Expr) : M σ (Option Expr) := do
   (← read).discharge? e
+
+def getConfig : M σ Config :=
+  return (← readThe Context).config
+
+@[inline] def withParent (parent : Expr) (f : M σ α) : M σ α :=
+  withTheReader Context (fun ctx => { ctx with parent? := parent }) f
 
 end Simp
 
